{
 "cells": [
  {
   "cell_type": "markdown",
   "metadata": {},
   "source": [
    "# 1 \n",
    "<b>If $A_n \\subset A_{n-1} \\subset \\dots \\subset A_1$ show that $\\cap_{i=1}^n A_i = A_n$, $\\cup_{i=1}^n A_i = A_1$ </b>\n",
    "\n",
    "We will prove it by induction over $n$ each one of the results.\n",
    "\n",
    "#### 1.1 $\\cup_{i=1}^n A_i = A_n$\n",
    "\n",
    "###### 1.1.1 Base case $n=2$\n",
    "\n",
    "For $n=2$ the hypothesis simplifies to:\n",
    "\\begin{equation*}\n",
    "A_2 \\subset A_1\n",
    "\\end{equation*}\n",
    "\n",
    "And the equality to prove simplifies to \n",
    "\n",
    "\\begin{equation*}\n",
    "A_1 \\cap A_2 = A_2\n",
    "\\end{equation*}\n",
    "\n",
    "In strict theory, for any set equality to be true, we would need to prove two things:\n",
    "\n",
    "\\begin{equation*}\n",
    "(A_1 \\cap A_2) \\subset A_2 \\;\\land\\; A_2 \\subset (A_1 \\cap A_2)\n",
    "\\end{equation*}\n",
    "\n",
    "In other words, we need to prove that any element of $(A_1 \\cap A_2)$ is also in $A_2$ and viceversa. Let us begin by proving the first part.\n",
    "\n",
    "Let $x \\in (A_1 \\cap A_2)$, by definition of set intersection we know that:\n",
    "\n",
    "\\begin{equation*}\n",
    "x \\in A_1 \\;\\land\\; x \\in A_2\n",
    "\\end{equation*}\n",
    "\n",
    "By the laws of logic, if the AND is true as a whole, we know that each individual operand is also true. In particular, we can tell that\n",
    "\n",
    "\\begin{equation*}\n",
    "x \\in A_2\n",
    "\\end{equation*}\n",
    "\n",
    "But if the $x$ is also in $A_2$, then by definition of $\\subset$ operator we can tell that $(A_1 \\cap A_2) \\subset A_2$; which is want we wanted to prove. \n",
    "\n",
    "Let us go now in the opposite direction, let us pick a $y \\in A_2$ and prove that $y$ also belongs to $(A_1 \\cap A_2)$. By hypothesis we know that $A_2 \\subset A_1$, hence $y \\in A_1$. So we have a couple of conditions holding now:\n",
    "\n",
    "<ol>\n",
    "<li> $y \\in A_2$ </li>\n",
    "<li> $y \\in A_1$ </li>\n",
    "</ol>\n",
    "\n",
    "But if both conditions above hold, is the same as having an AND over them:\n",
    "\n",
    "\\begin{equation*}\n",
    "y \\in A_1 \\;\\land\\; y \\in A_2\n",
    "\\end{equation*}\n",
    "\n",
    "And by definition of the intersection of sets, we know that $y \\in (A_1 \\cap A_2)$; which is the second part we needed to prove.\n",
    "\n",
    "Putting together:\n",
    "\n",
    "\\begin{equation*}\n",
    "(A_1 \\cap A_2) \\subset A_2 \\;\\land\\; A_2 \\subset (A_1 \\cap A_2) \n",
    "\\;\\;\\implies\\;\\; (A_1 \\cap A_2) = A_2\n",
    "\\end{equation*}\n",
    "\n",
    "and this proves the base case.\n",
    "\n",
    "###### 1.1.2 Inductive case $P(n) \\implies P(n+1)$\n",
    "\n",
    "For the inductive case, we will prove that assuming the property true for $n$, implies the property also holds for $n+1$ (in other words, we want to prove that the property is \"inherited\"). \n",
    "\n",
    "Let us look first at the induction hypothesis $P(n)$:\n",
    "\n",
    "\\begin{equation*}\n",
    "\\cap_{i=1}^n A_i = A_n\n",
    "\\end{equation*}\n",
    "\n",
    "and let us remember the additional hyphothesis for the exercise:\n",
    "\n",
    "\\begin{equation*}\n",
    "A_{n+1} \\subset A_n \\subset A_{n-1} \\subset \\dots \\subset A_1\n",
    "\\end{equation*}\n",
    "\n",
    "using the two hypothesis above we need to prove the property $P(n+1)$, which is:\n",
    "\n",
    "\\begin{equation*}\n",
    "\\cap_{i=1}^{n+1} A_i = A_{n+1}\n",
    "\\end{equation*}\n",
    "\n",
    "Let us begin with the left hand, and gradually transform it into the right hand, justifying the steps with the hypotheses that we mentioned.\n",
    "\n",
    "\\begin{align*}\n",
    "\\cap_{i=1}^{n+1} A_i &= (\\cap_{i=1}^{n} A_i) \\cap A_{n+1} \n",
    "& \\text{by associativity of $\\cap$} \\\\\n",
    "&= A_n \\cap A_{n+1} & \\text{by induction hypothesis} \\\\\n",
    "&= A_{n+1} & \\text{since $A_{n+1} \\subset A_n$, we use base case} \n",
    "\\end{align*}\n",
    "\n",
    "#### 1.2 $\\cup_{i=1}^n A_i = A_1$\n",
    "\n",
    "We will use same techniques as previous sub-exercise, but this time we will use more natural language instead of only mathematical notation. We will also omit some of the details, to make the proof briefer.\n",
    "\n",
    "###### 1.2.1 Base case $n=2$\n",
    "\n",
    "For $n=2$ the hyphothesis simplifies to:\n",
    "\\begin{equation*}\n",
    "A_2 \\subset A_1\n",
    "\\end{equation*}\n",
    "\n",
    "And the equality to prove simplifies to \n",
    "\n",
    "\\begin{equation*}\n",
    "A_1 \\cup A_2 = A_1\n",
    "\\end{equation*}\n",
    "\n",
    "Let us argument first why $(A_1 \\cup A_2) \\subset A_1$: let $x \\in A_1 \\cup A_2$; by definition of the set operator $\\cup$, the element $x$ belongs either to $A_1$, to $A_2$ or to both. If $x$ belongs to $A_1$ or to both, then the result holds immediately: the $x$ belongs to $A_1$. The remaining scenario is when $x \\in A_2$, and in that case we use the hipothesis $A_2 \\subset A_1$. This tells that any element of $A_2$ is also an element of $A_1$; hence $x \\in A_1$, which is what we wanted to prove.\n",
    "\n",
    "Let us argument now why $A_1 \\subset (A_1 \\cup A_2)$: let $y \\in A_1$, by definition of set operator $\\cup$, the element also belongs to $A_1 \\cup A_2$ (this is actually a propositional logic result: $p \\implies (p \\lor q))$. And that's it, having $y \\in A_1 \\cup A_2$ is what we wanted to prove.\n",
    "\n",
    "Together the two arguments above show that the sets are equal ($A_1 \\cup A_2 = A_1$), and this concludes our base case.\n",
    "\n",
    "\n",
    "###### 1.2.2 Inductive case\n",
    "\n",
    "The property for $n+1$ in this case is:\n",
    "\n",
    "\\begin{equation*}\n",
    "\\cup_{i=1}^{n+1} A_i = A_1\n",
    "\\end{equation*}\n",
    "\n",
    "Let us prove it again by starting with the left side, and gradually transform until we reach the right side (justifying each step):\n",
    "\n",
    "\\begin{align*}\n",
    "\\cup_{i=1}^{n+1} A_i &= A_1 \\cup (\\cup_{i=2}^{n+1} A_i) \n",
    "& \\text{by associativity of $\\cup$} \\\\\n",
    "&= A_1 \\cup A_2 & \\text{by induction hypothesis (right side has $n$ elements)} \\\\\n",
    "&= A_1 & \\text{since $A_2 \\subset A_1$, we use base case} \n",
    "\\end{align*}\n"
   ]
  },
  {
   "cell_type": "markdown",
   "metadata": {
    "collapsed": true
   },
   "source": [
    "# 2\n",
    "<b>If $X$ is the number of successes in $N$ Bernoulli trials, find the probability that $X >= 3$ given that $X >= 1$</b>\n",
    "\n",
    "Let us assign names to our events: \n",
    "\n",
    "<ul>\n",
    "<li>A := $X >= 3$</li>\n",
    "<li>B := $X >= 1$</li>\n",
    "</ul>\n",
    "\n",
    "Then this question is asking for the conditional probability $P(A \\mid B)$. We know that the definition of such is:\n",
    "\n",
    "\\begin{equation*}\n",
    "P(A \\mid B) = \\dfrac{P(A \\cap B)}{P(B)}\n",
    "\\end{equation*}\n",
    "\n",
    "Now, we can leverage the previous exercise's result because $A \\subset B$:\n",
    "\n",
    "\\begin{equation*}\n",
    "A \\subset B \\;\\implies\\; A \\cap B = A\n",
    "\\end{equation*}\n",
    "\n",
    "Then our conditional probability simplifies to:\n",
    "\n",
    "\\begin{equation*}\n",
    "P(A \\mid B) = \\dfrac{P(A)}{P(B)}\n",
    "\\end{equation*}\n",
    "\n",
    "All we need to do now, is to give a more concrete value to $P(A)$ and $P(B)$. Let us begin with $P(A)$:\n",
    "\n",
    "\\begin{align*}\n",
    "P(A) &= P(X >= 3) \\\\\n",
    "     &= 1 - P(X < 3) \\\\\n",
    "     &= 1 - \\left[ P(X=0) + P(X=1) + P(X=2) \\right] \\\\\n",
    "     &= 1 - P(X=0) - P(X=1) - P(X=2)\n",
    "\\end{align*}\n",
    "\n",
    "Similarly we proceed for $P(B)$:\n",
    "\n",
    "\\begin{align*}\n",
    "P(B) &= P(X >= 1) \\\\\n",
    "     &= 1 - P(X < 1) \\\\\n",
    "     &= 1 - P(X=0)\n",
    "\\end{align*}\n",
    "\n",
    "Thus, $P(A \\mid B)$ becomes:\n",
    "\n",
    "\\begin{equation*}\n",
    "P(A \\mid B) = \\dfrac{P(X >= 3)}{P(X >= 1)} = \n",
    "\\dfrac{1 - P(X=2) - P(X=1) - P(X=0)}{1 - P(X=0)}\n",
    "\\end{equation*}\n",
    "\n",
    "But given these are $n$ Bernoulli trials, we actually know the definition of $P(X=k)$:\n",
    "\n",
    "\\begin{equation*}\n",
    "P(X=k) = C^n_k p^k q^{n-k}\n",
    "\\end{equation*}\n",
    "\n",
    "Let us apply this definition to our terms $P(X=k)$:\n",
    "\n",
    "\\begin{align*}\n",
    "P(X=0) &= C^n_0 p^0 q^{n-0} = q^n \\\\\n",
    "P(X=1) &= C^n_1 p^1 q^{n-1} = n p q^{n-1} \\\\\n",
    "P(X=2) &= C^n_2 p^2 q^{n-2} \n",
    "\\end{align*}\n",
    "\n",
    "Let us substitute now in our formula for $P(A|B)$ to yield the final result (alright, let us actually summarize the whole development):\n",
    "\n",
    "\\begin{align*}\n",
    "P(A \\mid B) \n",
    "&= \\dfrac{P(A \\cap B)}{P(B)} \\\\\\\\\n",
    "&= \\dfrac{P(\\{X >= 3\\} \\cap \\{X >= 1\\})}{P(X >= 1)} \\\\\\\\\n",
    "&= \\dfrac{P(X >= 3)}{P(X >= 1)} \\\\\\\\ \n",
    "&= \\dfrac{1 - P(X=2) - P(X=1) - P(X=0)}{1 - P(X=0)} \\\\\\\\\n",
    "&= \\dfrac{1 - C^n_2 p^2 q^{n-2} - n p q^{n-1} - q^n}{1 -q^n} \n",
    "\\end{align*}\n"
   ]
  },
  {
   "cell_type": "markdown",
   "metadata": {},
   "source": [
    "# 3\n",
    "<b>Let $C_1$ be an unbiased coin, and $C_2$ a biased coin with probability of heads $\\frac{3}{4}$. At time $t = 0$, $C_1$ is tossed. If the result is heads, then $C_1$ is tossed at time $t = 1$. If the result is tails, $C_2$ is tossed at $t = 1$. Then the process is repeated at time $t = 2, 3, \\dots$. In general, if heads appears at $t = n$, then $C_1$ is tossed at time $t = n+1$. If tails appears at $t = n$, then $C_2$ is tossed at $t = n+1$.</b>\n",
    "\n",
    "<b>Find $y_n$ = the probability that the toss at $t = n$ will be head (hint: use a difference equation)</b>\n",
    "\n",
    "We can use the law of total probability, at time $n$. What occurs there, depends on what happened on time $n-1$ (aka $y_{n-1}$), but split in two disjoint cases. This is because depending on whether we got head or tail a time $n-1$, we used either coin $C_1$ or $C_2$. And for each coin, we know that the conditional probability of getting head is different. Thus, the recurrence relation can be explained as follows:\n",
    "\n",
    "At time $n$, the probability of getting head is given by the sum of two probabilities: the probability of getting head at time $n-1$ times the probability of getting head on $C_1$; plus the probability of getting tail at time $n-1$ times the probability of getting head on $C_2$.\n",
    "\n",
    "Let $H$ be the probability of getting head, our recurrence equation can be written formally as:\n",
    "\n",
    "\\begin{align*}\n",
    "y_n &= y_{n-1} P(H \\mid C_1) + (1 - y_{n-1})P(H \\mid C_2) \\\\\n",
    "    &= y_{n-1} \\frac{1}{2} + (1 - y_{n-1})\\frac{3}{4} \\\\\n",
    "    &= y_{n-1} \\frac{1}{2}  - y_{n-1}\\frac{3}{4} + \\frac{3}{4} \\\\\n",
    "    &= - \\frac{y_{n-1}}{4} + \\frac{3}{4} \\\\\n",
    "\\end{align*}\n",
    "\n",
    "Our recurrence relation can actually be seen as a recurrence equation:\n",
    "\n",
    "\\begin{equation*}\n",
    "y_n + \\frac{y_{n-1}}{4} = \\frac{3}{4} \n",
    "\\end{equation*}\n",
    "\n",
    "Recurrence equations are the discrete counterpart of differencial equations, and this particular specimen is an inhomogeneus first order linear difference equation. The general recipe for solving those is as follows:\n",
    "\n",
    "<ol>\n",
    "<li>Find a particular solution for inhomogeneous equation.</li>\n",
    "<li>Find the general solution for the associated homogeneous equation.</li>\n",
    "<li>The general solution for inhomogeneous equation, is the sum of the two above.</li>\n",
    "<li>Using initial conditions we can resolve parameters.</li>\n",
    "</ol>\n",
    "\n",
    "Let us begin by finding a particular solution for the inhomogeneous equation. Given that the right hand is constant, we can assume the particular solution is constant as well. This means that:\n",
    "\n",
    "\\begin{equation*}\n",
    "y_{n} = y_{n-1} = c\n",
    "\\end{equation*}\n",
    "\n",
    "Replacing the constant on the difference equation gives us:\n",
    "\n",
    "\\begin{align*}\n",
    "c + \\frac{c}{4} &= \\frac{3}{4} \\implies \\\\\n",
    "\\frac{5c}{4} &= \\frac{3}{4} \\implies \\\\\n",
    "5c &= 3 \\implies \\\\\n",
    "c &= \\frac{3}{5} \n",
    "\\end{align*}\n",
    "\n",
    "Then, our particular solution is constant $y_n = \\frac{3}{5}$. Let us find now the general solution for the homogeneous equation:\n",
    "\n",
    "\\begin{equation*}\n",
    "y_n + \\frac{y_{n-1}}{4} = 0\n",
    "\\end{equation*}\n",
    "\n",
    "The generic solution for such equation is given by:\n",
    "\n",
    "\\begin{equation*}\n",
    "y_n = K \\left(-\\frac{1}{4}\\right)^n\n",
    "\\end{equation*}\n",
    "\n",
    "And thus, adding both together, leads to general solution for the inhomogeneus equation:\n",
    "\n",
    "\\begin{equation*}\n",
    "y_n = K \\left(-\\frac{1}{4}\\right)^n + \\frac{3}{5}\n",
    "\\end{equation*}\n",
    "\n",
    "Where the constant $K$ can be known by using initial conditions. We know what is $y_0$, because the problem says that at $t = 0$ we toss coin $C_1$; and thus:\n",
    "\n",
    "\\begin{equation*}\n",
    "y_0 = P(H \\mid C_1) = \\frac{1}{2}\n",
    "\\end{equation*}\n",
    "\n",
    "Replacing above value for $y_0$ into general solution, allows to find what is $K$:\n",
    "\n",
    "\\begin{align*}\n",
    "y_0 &= K \\left(-\\frac{1}{4}\\right)^0 + \\frac{3}{5} \\implies \\\\\n",
    "\\frac{1}{2} &= K + \\frac{3}{5} \\implies \\\\\n",
    "K  &= \\frac{1}{2} - \\frac{3}{5} = -\\frac{1}{10}\n",
    "\\end{align*}\n",
    "\n",
    "Therefore, the final solution for inhomogeneous equation would be the following:\n",
    "\n",
    "\\begin{equation*}\n",
    "y_n = -\\frac{1}{10} \\left(-\\frac{1}{4}\\right)^n + \\frac{3}{5}\n",
    "\\end{equation*}\n",
    "\n",
    "which is the probability we were asked for.\n"
   ]
  },
  {
   "cell_type": "markdown",
   "metadata": {
    "collapsed": true
   },
   "source": [
    "# 4\n",
    "<b>Consider a sequence of five Bernoulli trials. Let $R$ be the number of times a head is followed immediately by a tail. For example, if $w = HHTHT$, then $R(w)=2$ since a head is followed by a tail at trials 2 and 3, and also at trials 4 and 5. Find the probability function of $R$</b>\n",
    "\n",
    "Given the constraint of 5 trails, we know that the random variable $R$ can only have values in $\\{0, 1, 2\\}$. Furthermore, there are a total of $2^5 = 32$ possible final configurations; and they will be grouped according to the values of $R$. Let us proceed to count them all manually, they are not that many. For each configuration we will also list its probability of ocurrence (where $p$ is the probability of success/head, and $q$ is probability of failure/tail).\n",
    "\n",
    "The possible configurations with $R=0$:\n",
    "\n",
    "<table>\n",
    "<tr><td>$HHHHH$</td><td>$p^5$</td></tr>\n",
    "<tr><td>$HHHHT$</td><td>$p^4q$</td></tr>\n",
    "<tr><td>$HHHTT$</td><td>$p^3q^2$</td></tr>\n",
    "<tr><td>$HHTTT$</td><td>$p^2q^3$</td></tr>\n",
    "<tr><td>$HTTTT$</td><td>$pq^4$</td></tr>\n",
    "<tr><td>$TTTTT$</td><td>$q^5$</td></tr>\n",
    "</table>\n",
    "\n",
    "The possible configurations with $R=1$:\n",
    "\n",
    "<table>\n",
    "<tr><td>$HHHHT$</td><td>$p^4q$</td></tr>\n",
    "<tr><td>$HHHTH$</td><td>$p^4q$</td></tr>\n",
    "<tr><td>$HHTHH$</td><td>$p^4q$</td></tr>\n",
    "<tr><td>$HTHHH$</td><td>$p^4q$</td></tr>\n",
    "<tr><td>$HHHTT$</td><td>$p^3q^2$</td></tr>\n",
    "<tr><td>$HHTTH$</td><td>$p^3q^2$</td></tr>\n",
    "<tr><td>$HTTHH$</td><td>$p^3q^2$</td></tr>\n",
    "<tr><td>$THHHT$</td><td>$p^3q^2$</td></tr>\n",
    "<tr><td>$THHTH$</td><td>$p^3q^2$</td></tr>\n",
    "<tr><td>$THTHH$</td><td>$p^3q^2$</td></tr>\n",
    "<tr><td>$HHTTT$</td><td>$p^2q^3$</td></tr>\n",
    "<tr><td>$HTTTH$</td><td>$p^2q^3$</td></tr>\n",
    "<tr><td>$THHTT$</td><td>$p^2q^3$</td></tr>\n",
    "<tr><td>$THTTH$</td><td>$p^2q^3$</td></tr>\n",
    "<tr><td>$TTHHT$</td><td>$p^2q^3$</td></tr>\n",
    "<tr><td>$TTHTH$</td><td>$p^2q^3$</td></tr>\n",
    "<tr><td>$HTTTT$</td><td>$pq^4$</td></tr>\n",
    "<tr><td>$THTTT$</td><td>$pq^4$</td></tr>\n",
    "<tr><td>$TTHTT$</td><td>$pq^4$</td></tr>\n",
    "<tr><td>$TTTHT$</td><td>$pq^4$</td></tr>\n",
    "</table>\n",
    "\n",
    "And these are the configurations for $R=2$:\n",
    "\n",
    "<table>\n",
    "<tr><td>$HHTHT$</td><td>$p^3q^2$</td></tr>\n",
    "<tr><td>$HTHTH$</td><td>$p^3q^2$</td></tr>\n",
    "<tr><td>$HTHHT$</td><td>$p^3q^2$</td></tr>\n",
    "<tr><td>$THTHT$</td><td>$p^2q^3$</td></tr>\n",
    "<tr><td>$HTHTT$</td><td>$p^2q^3$</td></tr>\n",
    "<tr><td>$HTTHT$</td><td>$p^2q^3$</td></tr>\n",
    "</table>\n",
    "\n",
    "If the coin was known to be unbiased, then we could assume that all the 32 configurations have the same probability; hence we could simply say:\n",
    "\n",
    "\\begin{equation*}\n",
    "P(R=0) = \\frac{6}{32} \\\\\n",
    "P(R=1) = \\frac{20}{32} \\\\\n",
    "P(R=2) = \\frac{6}{32} \n",
    "\\end{equation*}\n",
    "\n",
    "But since we do not know if the coin is unbiased, we need to answer this question in terms of $p$ and $q$. For this purpose, we just need to sum all the probabilities for each configuration; as they are already grouped per value of $R$. Let us note that within each group, the configurations are already sorted by pattern $p^kq^{5-k}$. This was done to make the next task easier, so we can quickly count the size of each sub-group:\n",
    "\n",
    "\\begin{align*}\n",
    "P(R=0) &= \\sum_{k=0}^5 p^kq^{5-k} \\\\\\\\\n",
    "P(R=1) &= 4p^4q + 6p^3q^2 + 6p^2q^3 + 4pq^4 \\\\\\\\\n",
    "P(R=2) &= 3p^3q^2 + 3p^2q^3\n",
    "\\end{align*}\n",
    "\n",
    "Above is the requested probability (density) function for random variable $R$."
   ]
  },
  {
   "cell_type": "markdown",
   "metadata": {
    "collapsed": true
   },
   "source": [
    "# 5\n",
    "<b>An employer is about to hire one new employee from a group of $N$ candidates, whose future potential can be rated on a scale from $1$ to $N$. The employer proceeds according to the following rules:</b>\n",
    "\n",
    "<b>(a) Each candidate is seen in succession (in random order) and a decision is made whether to hire the candidate.</b>\n",
    "\n",
    "<b>(b) Having rejected $m-1$ candidates ($m > 1$), the employer can hire the $m_{th}$ candidate only if the $m_{th}$ candidate is better than the previous $m-1$.</b>\n",
    "\n",
    "<b>Suppose a candidate is hired on the $i_{th}$ trial. What is the probability that the best candidate was hired?</b>\n",
    "\n",
    "The rule (a) pretty much tells us that the candidates are to be taken from a shuffled array. The resulting random permutation could be any, and we know that a hiring decision was made at position $i$ (our index starts at $1$). \n",
    "\n",
    "The rule (b) tells us that the previous $i-1$ candidates had a lower ranking, so we can conclude that best guy was not among them. This means that the best candidate must have an index from the set:\n",
    "\n",
    "\\begin{equation*}\n",
    "\\{ i, i+1, i+2, \\cdots, N \\}\n",
    "\\end{equation*}\n",
    "\n",
    "The size of the previous set is $N - (i-1)$, because we are discounting the rejected $i-1$ folks who are worse than candidate $i$. Thus, from this remaining set any guy could be the best; that is, the probability that any of those indexes to correspond to best candidate is:\n",
    "\n",
    "\\begin{equation*}\n",
    "P(\\text{any remaining index to be the best}) = \n",
    "\\frac{1}{N-(i-1)} = \n",
    "\\frac{1}{N-i+1}\n",
    "\\end{equation*}\n",
    "\n",
    "Above reasoning applies in particular to the chosen candidate $i$, hence the probability of having hired the best candidate is given by:\n",
    "\n",
    "\\begin{equation*}\n",
    "P(\\text{best candidate being at index } i) = \n",
    "\\frac{1}{N-i+1}\n",
    "\\end{equation*}\n",
    "\n"
   ]
  },
  {
   "cell_type": "code",
   "execution_count": null,
   "metadata": {
    "collapsed": true
   },
   "outputs": [],
   "source": []
  }
 ],
 "metadata": {
  "kernelspec": {
   "display_name": "Python 2",
   "language": "python",
   "name": "python2"
  },
  "language_info": {
   "codemirror_mode": {
    "name": "ipython",
    "version": 2
   },
   "file_extension": ".py",
   "mimetype": "text/x-python",
   "name": "python",
   "nbconvert_exporter": "python",
   "pygments_lexer": "ipython2",
   "version": "2.7.13"
  }
 },
 "nbformat": 4,
 "nbformat_minor": 2
}
