---
output:
  pdf_document: default
  html_document: default
geometry: margin=1cm
---

\pagenumbering{gobble}
Prove that

\[
\frac{\partial J}{\partial u_w} = 
\begin{cases}
(\hat{y}_w - 1)v_c & \text{if } w = o \\
\hat{y}_w v_c & \text{otherwise}
\end{cases}
\]

Proof (tried to reuse previous answer as much as possible):

\begin{align*}
J_{naive-softmax}(v_c, o, U) &= -u_o^T v_c + 
log \left(\sum_{w' \in Vocab} exp(u_{w'}^T v_c)\right) \\\\
\frac{\partial J}{\partial u_w} &= \frac{\partial}{\partial u_w} \left( -u_o^T v_c + log\left(\sum_{w' \in Vocab} exp(u_{w'}^T v_c)\right)\right) && \text{taking derivative on both sides} \\\\
&= \frac{\partial}{\partial u_w} \left( -u_o^T v_c \right) +  \frac{\partial}{\partial u_w} \left( log\left(\sum_{w' \in Vocab} exp(u_{w'}^T v_c)\right)\right) && \text{derivative of a sum} \\\\
&= \frac{\partial}{\partial u_w} \left( -u_o^T v_c \right) +  \dfrac{\frac{\partial}{\partial u_w} \left( \sum_{w' \in Vocab} exp(u_{w'}^T v_c)\right)}{\sum_{w' \in Vocab} exp(u_{w'}^T v_c)} && \text{derivative of log} \\\\
&= \frac{\partial}{\partial u_w} \left( -u_o^T v_c \right) +  \dfrac{\sum_{w' \in Vocab} \frac{\partial}{\partial u_w} \left(exp(u_{w'}^T v_c)\right)}{\sum_{w' \in Vocab} exp(u_{w'}^T v_c)} && \text{derivative of a sum} \\\\
&= \frac{\partial}{\partial u_w} \left( -u_o^T v_c \right) +  \sum_{w' \in Vocab} \left(\dfrac{\frac{\partial}{\partial u_w} \left(exp(u_{w'}^T v_c)\right)}{\sum_{w'' \in Vocab} exp(u_{w''}^T v_c)}\right) && \text{re-arranging the sum and renaming index} \\\\
&= \frac{\partial}{\partial u_w} \left( -u_o^T v_c \right) +  \sum_{w' \in Vocab} \left(\dfrac{exp(u_{w'}^T v_c) \frac{\partial}{\partial u_w} \left( u_{w'}^T v_c \right) }{\sum_{w'' \in Vocab} exp(u_{w''}^T v_c)}\right) && \text{derivative of exp} \\\\
&= \frac{\partial}{\partial u_w} \left( -u_o^T v_c \right) +  \dfrac{exp(u_w^T v_c) \frac{\partial}{\partial u_w} \left( u_{w}^T v_c \right) }{\sum_{w'' \in Vocab} exp(u_{w''}^T v_c)} && \frac{\partial}{\partial u_w} \left( u_{w'}^T v_c \right) = 0\;\;, \forall w' \neq w \\\\
&= \frac{\partial}{\partial u_w} \left( -u_o^T v_c \right) +   \dfrac{exp(u_w^T v_c) v_c }{\sum_{w'' \in Vocab} exp(u_{w''}^T v_c)} && \frac{\partial}{\partial u_w} \left( u_{w}^T v_c \right) = v_c \\\\
&= \frac{\partial}{\partial u_w} \left( -u_o^T v_c \right) +   \left(\dfrac{exp(u_w^T v_c)}{\sum_{w'' \in Vocab} exp(u_{w''}^T v_c)}\right) v_c && \text{associativity law} \\\\
&=  \frac{\partial}{\partial u_w}\left(-u_o^T v_c \right) + 
\hat{y}_w v_c && \text{definition of } \hat{y}_w  \\\\
&= \hat{y}_w v_c - \frac{\partial}{\partial u_w} \left(u_o^T v_c \right) && \text{commutativity and sign laws} \\\\
&= \begin{cases}
\hat{y}_w v_c - \frac{\partial}{\partial u_o} \left(u_o^T v_c \right) & \text{if } w = o \\
\hat{y}_w v_c - \frac{\partial}{\partial u_w} \left(u_o^T v_c \right) & \text{otherwise}
\end{cases} &&  \text{Analysis by cases} \\\\
&= \begin{cases}
\hat{y}_w v_c - v_c & \text{if } w = o \\
\hat{y}_w v_c - 0 & \text{otherwise}
\end{cases} &&  \text{Derivative of $xa$ and $ba$ respect to $x$} \\\\
&= \begin{cases}
(\hat{y}_w - 1)v_c & \text{if } w = o \\
\hat{y}_w v_c & \text{otherwise}
\end{cases} && \text{distributivity law and additive identity}\;\; \square
\end{align*}
